HOL/Set_Thms.thy
@@ -108,10 +108,19 @@ setup {* add_forward_prfstep_cond @{thm member_notin_contra} [with_term "?S - {?
 
 subsection {* Results on finite sets *}
 
+setup {* add_property_const @{term finite} *}
 setup {* add_resolve_prfstep @{thm Finite_Set.finite.emptyI} *}
-theorem set_finite_single [resolve]: "finite {x}" by simp
+lemma set_finite_single [resolve]: "finite {x}" by simp
 setup {* add_rewrite_rule @{thm Finite_Set.finite_Un} *}
-theorem Max_ge' [forward]: "finite A \<Longrightarrow> x > Max A \<Longrightarrow> \<not>(x \<in> A)" using Max_ge leD by auto
+lemma Max_ge' [forward]: "finite A \<Longrightarrow> x > Max A \<Longrightarrow> \<not>(x \<in> A)" using Max_ge leD by auto
+
+subsection {* Cardinality *}
+
+setup {* add_rewrite_rule @{thm card_empty} *}
+lemma card_emptyD [rewrite]: "finite S \<Longrightarrow> card S = 0 \<Longrightarrow> S = {}" by simp
+lemma card_minus1 [rewrite]:
+  "x \<in> S \<Longrightarrow> card (S - {x}) = card S - 1" by (simp add: card_Diff_subset)
+setup {* add_forward_prfstep @{thm finite_Diff} *}
 
 subsection {* image_set *}
 
